\section{Testing provenance semantics across different semirings of interest}
\subsection{counting semiring}
$$k = (\mathbb{n}, \oplus, \otimes, 0, 1)$$
$\mathbb{n} = \{0,1,2,\dots\}$

$\oplus : \text{standard integer addition}$

$\otimes : \text{standard integer multiplication}$

$\text{zero} : 0 \in \mathbb{n}$

$\text{one} : 1 \in \mathbb{n}$

additional operators:

monus: $(a \ominus b): \text{truncated subtraction}$
$$ a \ominus b = \begin{cases} 0, &  a\leq b\\ a-b,& a>b \end{cases}$$

delta: 
for $a \in k$
$\delta(a) = \begin{cases} 0, & a=0\\ 1, & a>0 \end{cases}$
$\delta:k \mapsto k $
$\delta(0_k)=0_k$
$\delta(n.1_k)=1_k$


\textbf{counting semiring properties:}

1. additive monoid
- associativity: $$(a \oplus b) \oplus c = a \oplus (b\oplus c)$$
- commutativity: $$a \oplus b = b \oplus a$$
- identity: $$a \oplus 0 = 0$$
2. Multiplicative monoid
- Associativity: $$( (a \otimes b) \otimes c = a \otimes (b\otimes c)$$
- Commutativity: $$a \otimes b = b \otimes a$$
- Identity: $$a \otimes 1 = a$$
3. Distributivity
- Left Dist: $$a \otimes (b \oplus c)= (a \otimes b)\oplus(a \otimes c)$$
- RIght Dist: $$(a \oplus b)\otimes c=(a \otimes c)\oplus(b \otimes c)$$
 4. Absorption
$$a \otimes 0 = 0 \otimes a = 0$$

5. Monus \newline
For $$a, b \in K$$
- $$(a \ominus b) \oplus b =a$$, if $$a \geq b$$
- $$a \ominus 0 =a$$
- $$0 \ominus a = 0$$

6. Semimodule operation
- Associative with semiring multiplication: $$a \otimes (b * m)= (a \otimes b) * m$$
- Identity: $$1*m=m$$
- Absorption: $$0*m=0$$
7. Other properties
$$
 \delta(u)\otimes[[u \oslash   v]]_{\mathit{op}}=\begin{cases}1, & \text{if } u\hspace{0.5em} op\hspace{0.5em} v \text{ holds in } \mathbb{N} \\
0,&\text{o.w.}\end{cases}
$$

e.g. For COUNT(*), say we have $f=\bigoplus_{g \in group}$ 1 and we want to filter on the aggregates HAVING >C

$$
 \delta(f)\otimes[[f \oslash   C]]_{\mathit{>}}=\begin{cases}1, & \text{if } f>C \text{ holds in } \mathbb{N} \\
0,&\text{o.w.}\end{cases}
$$

\subsection{Boolean Semiring}
$$B = (\{0,1\}, \lor, \land, 0, 1)$$
$$\lor : \text{Standard logical OR}$$
$$\land : \text{Standard logical AND}$$
$$0 : \text{Boolean zero}$$
$$1 : \text{Boolean one}$$
\[
\ominus: \text{Monus for Boolean Semiring} \quad a \ominus b := a \land \neg b
\]
Now we take a query as below on a relation $T$ with $n$ tuples:

\begin{listing}[ht]
\begin{minted}[linenos,frame=single,fontsize=\small]{sql}
SELECT DISTINCT 1
  FROM T
 HAVING COUNT(*) = c;
\end{minted}
\end{listing}

This returns 1 if the relation $T$ has exactly $c$ tuples, and 0 otherwise.

In possible world semantics, let $w: \{1,2,\dots,m\} \mapsto \{0,1\}$.

The provenance of this query can be expressed as follows:

$$q(T) = \bigoplus_{w}\left(\bigotimes_{w(i)=1}b_i\otimes\left(\mathbb{1}\ominus(\bigoplus_{w(i) =0}b_i)\right)\right)$$

On the other hand, its equivalent join query will be as follows:

\begin{listing}[ht]
\caption{Return 1 if \(|T| = c\) using joins on distinct rows}
\begin{minted}[linenos,frame=single,fontsize=\small]{sql}
SELECT DISTINCT 1
  FROM T AS a1
  JOIN T AS a2 ON a1.id <  a2.id
  JOIN T AS a3 ON a2.id <  a3.id
  -- ...
  JOIN T AS a_c ON a_{c-1}.id < a_c.id

EXCEPT

SELECT DISTINCT 1
  FROM T AS b1
  JOIN T AS b2 ON b1.id <  b2.id
  JOIN T AS b3 ON b2.id <  b3.id
  -- ...
  JOIN T AS b_{c+1} ON b_c.id < b_{c+1}.id;
\end{minted}
\end{listing}

The provenance of this query can be expressed as follows:
\[
q'(T) = \bigoplus_{\substack{t\subseteq T \\ |t| = c}}\left(\bigotimes_{\substack{b_i\in t}}b_i\right) \ominus \bigoplus_{\substack{t'\subseteq T \\ |t'| = c+1}}\left(\bigotimes_{\substack{b_i\in t'}}b_i\right)
\]

\begin{proof}
Define
\[
A \;=\; \bigvee_{\lvert t\rvert = c}\;\bigwedge_{i\in t} b_i,
\qquad
B \;=\; \bigvee_{\lvert t'\rvert = c+1}\;\bigwedge_{i\in t'} b_i.
\]
Since in the Boolean semiring \(\oplus=\vee\), \(\otimes=\wedge\) and
\(\;r\ominus s = r\wedge\neg s\), we have
\[
q'(T)
= A \ominus B
= A \wedge \neg B.
\]
Expand step by step:
\begin{align*}
q'(T)
&= \Bigl(\!\bigvee_{\lvert t\rvert = c}\!\bigwedge_{i\in t}b_i\Bigr)
   \;\wedge\;
   \neg\Bigl(\!\bigvee_{\lvert t'\rvert = c+1}\!\bigwedge_{i\in t'}b_i\Bigr)\\[6pt]
&= \Bigl(\!\bigvee_{\lvert t\rvert = c}\!\bigwedge_{i\in t}b_i\Bigr)
   \;\wedge\;
   \Bigl(\!\bigwedge_{\lvert t'\rvert = c+1}\!\neg\bigl(\!\bigwedge_{i\in t'}b_i\bigr)\Bigr)\\[6pt]
&= \bigvee_{\lvert t\rvert = c}
    \Bigl(
      \bigwedge_{i\in t}b_i
      \;\wedge\;
      \bigwedge_{|t'|=c+1}\!\neg\bigl(\!\bigwedge_{i\in t'}b_i\bigr)
    \Bigr).
\end{align*}

\textbf{Key simplification.}  Fix a particular \(t\) with \(\lvert t\rvert=c\).  Consider
\[
\bigwedge_{\substack{t'\subseteq[m]\\|t'|=c+1}}
\neg\Bigl(\!\bigwedge_{i\in t'}b_i\Bigr).
\]
- For each \(j\notin t\), the subset \(t'=t\cup\{j\}\) yields
  \(\neg\bigl(b_j\wedge\bigwedge_{i\in t}b_i\bigr)=\neg b_j\).  
- Any other \(t'\) also contains some \(j\notin t\), so its factor
  \(\neg(\bigwedge_{i\in t'}b_i)\) can be written as
  \(\neg b_j\vee Y\).  

with \(x=\neg b_j\), each such pair of factors collapses to \(\neg b_j\).  Hence the entire
AND reduces to
\(\bigwedge_{j\notin t}\neg b_j\).

Substituting back gives
\[
q'(T)
=\bigvee_{\lvert t\rvert = c}
\Bigl(\,\bigwedge_{i\in t}b_i
       \;\wedge\;
       \bigwedge_{j\notin t}\neg b_j
\Bigr)
=\;q(T),
\]
as required.
\end{proof}
\input{homomorphisms.tex}
